Add provenance information to Composition
Initial state relations are extended with the missing parameters, which
are always in scope, and these are in turn propagated. In the standing
proofs, it suffices to reason by existing assumptions and the symmetry
of the provenance relation on mergeable interfaces.

Intermediate/Composition.v
@@ -1024,7 +1024,7 @@ Section Semantics.
 
   Inductive initial_state : PS.state -> Prop :=
   | initial_state_intro: forall ics ips,
-      CS.comes_from_initial_state ics ->
+      CS.comes_from_initial_state ics (unionm (prog_interface prog) ctx) ->
       PS.partial_state ctx ics ips ->
       PS.is_program_component ips ctx ->
       initial_state ips.
@@ -1060,7 +1060,7 @@ Section Semantics.
 
   Inductive initial_state : PS.state -> Prop :=
   | initial_state_intro: forall ics ips,
-      CS.comes_from_initial_state ics ->
+      CS.comes_from_initial_state ics (unionm (prog_interface prog) ctx) ->
       PS.partial_state ctx ics ips ->
       PS.is_context_component ips ctx ->
       initial_state ips.
@@ -1141,12 +1141,12 @@ Section Simulation.
     Regardless, observe that there remains a troublesome case when matching the
     PC form against mergeable_states.
 
-    Observe several goals repeat: pose, refactor, etc. *)
+    Observe several goals repeat: pose, refactor, etc. *) Print ProgramSem.initial_state.
   Lemma match_initial_states:
     forall ips1,
-      ProgramSem.initial_state (prog_interface c) ips1 ->
+      ProgramSem.initial_state p (prog_interface c) ips1 ->
     exists ips2,
-      ContextSem.initial_state (prog_interface p) ips2 /\
+      ContextSem.initial_state c (prog_interface p) ips2 /\
       PS.mergeable_states (prog_interface c) (prog_interface p) ips1 ips2.
   Proof.
     intros ips1 Hini.
@@ -1162,7 +1162,7 @@ Section Simulation.
           filterm (fun (k : nat) (_ : ComponentMemory.t) => k \notin domm (prog_interface p)) mem)).
     split.
     - econstructor.
-      + eassumption.
+      + apply CS.comes_from_initial_state_mergeable_sym; eassumption.
       + constructor.
         * PS.simplify_turn. eapply domm_partition; eassumption.
         * reflexivity.
@@ -1170,8 +1170,8 @@ Section Simulation.
       + PS.simplify_turn. eapply domm_partition; eassumption.
     - econstructor.
       + eapply mergeable_interfaces_sym; eassumption.
+      + apply CS.comes_from_initial_state_mergeable_sym; eassumption.
       + eassumption.
-      + assumption.
       + constructor.
         * PS.simplify_turn. eapply domm_partition; eassumption.
         * reflexivity.
@@ -1338,9 +1338,9 @@ Section Simulation.
 
   Lemma match_initial_states:
     forall ips1,
-      ContextSem.initial_state (prog_interface c) ips1 ->
+      ContextSem.initial_state p (prog_interface c) ips1 ->
     exists ips2,
-      ProgramSem.initial_state (prog_interface p) ips2 /\
+      ProgramSem.initial_state c (prog_interface p) ips2 /\
       PS.mergeable_states (prog_interface c) (prog_interface p) ips1 ips2.
   Proof.
     intros ips1 Hini.
@@ -1358,7 +1358,7 @@ Section Simulation.
           regs, pc)).
     split.
     - econstructor.
-      + eassumption.
+      + apply CS.comes_from_initial_state_mergeable_sym; eassumption.
       + constructor.
         * PS.simplify_turn. eapply PS.domm_partition_notin; eassumption.
         * reflexivity.
@@ -1366,7 +1366,7 @@ Section Simulation.
       + PS.simplify_turn. eapply PS.domm_partition_notin; eassumption.
     - econstructor.
       + eapply mergeable_interfaces_sym; eassumption.
-      + eassumption.
+      + apply CS.comes_from_initial_state_mergeable_sym; eassumption.
       + assumption.
       + constructor.
         * PS.simplify_turn. eapply PS.domm_partition_notin; eassumption.
